add a top-level to HSL and some other tweaks

examples/low-mitls-experiments/HSL.fst
@@ -5,11 +5,10 @@ module HSL
  *)
 
 open LowStar.ModifiesPat
-
-open FStar.UInt32
-
+open FStar.Integers
 open FStar.HyperStack
 open FStar.HyperStack.ST
+open LowStar.BufferOps
 
 module Mods   = LowStar.Modifies
 module Buffer = LowStar.Buffer
@@ -29,29 +28,29 @@ type loc = LowStar.Modifies.loc
  * So, the record layer appends to the buffer after p1
  * At some point (in HSL.process), HSL decides that the contents between p0 and p1 is a valid message
  * And at that point, it moves p0 and p1
- * 
+ *
  * We also keep msgs: list of all subsequences in the buffer that don't contain a 0ul
  *)
 abstract noeq type hsl_state =
-  | Mk_state: len:u32 ->
-              buf:Buffer.buffer u32{Buffer.len buf == len} ->
-              p0:reference u32 ->
-	      p1:reference u32 ->
-	      msgs:reference (list (u32 * u32)) ->
-	      hsl_state
+  | Mk_state: len:uint_32 ->
+              buf:Buffer.buffer uint_32{Buffer.len buf == len} ->
+              p0:reference uint_32 ->
+              p1:reference uint_32 ->
+              msgs:reference (list (uint_32 & uint_32)) ->
+              hsl_state
 
 (* abstract getters *)
-abstract let hsl_get_len (st:hsl_state) :u32 = st.len
-abstract let hsl_get_buf (st:hsl_state) :Buffer.buffer u32 = st.buf
-abstract let hsl_get_p0 (st:hsl_state) :reference u32 = st.p0
-abstract let hsl_get_p1 (st:hsl_state) :reference u32 = st.p1
-abstract let hsl_get_msgs (st:hsl_state) :reference (list (u32 * u32)) = st.msgs
+abstract let hsl_get_len (st:hsl_state) :uint_32 = st.len
+abstract let hsl_get_buf (st:hsl_state) :Buffer.buffer uint_32 = st.buf
+abstract let hsl_get_p0 (st:hsl_state) :reference uint_32 = st.p0
+abstract let hsl_get_p1 (st:hsl_state) :reference uint_32 = st.p1
+abstract let hsl_get_msgs (st:hsl_state) :reference (list (uint_32 & uint_32)) = st.msgs
 
 (* Liveness and disjointness *)
 [@"opaque_to_smt"]
 unfold private let liveness_and_disjointness (st:hsl_state) (h:mem) :Type0 =
   let len, buf, p0, p1, msgs = hsl_get_len st, hsl_get_buf st, hsl_get_p0 st, hsl_get_p1 st, hsl_get_msgs st in
-  
+
   loc_pairwise_disjoint [
     Mods.loc_mreference p0;
     Mods.loc_mreference p1;
@@ -61,8 +60,8 @@ unfold private let liveness_and_disjointness (st:hsl_state) (h:mem) :Type0 =
 
   Buffer.live h buf /\ contains h p0 /\ contains h p1 /\ contains h msgs /\  //liveness
   Buffer.len buf == len /\  //buffer length
-  sel h p1 <=^ len /\  //p1 is leq len
-  sel h p0 <=^ sel h p1  //p0 is leq p1
+  sel h p1 <= len /\  //p1 is leq len
+  sel h p0 <= sel h p1  //p0 is leq p1
 
 (*
  * An invariant on the sequence content between p0 and p1 in the buffer, that it doesn't contains 0ul
@@ -70,10 +69,13 @@ unfold private let liveness_and_disjointness (st:hsl_state) (h:mem) :Type0 =
  *)
 [@"opaque_to_smt"]
 unfold private let null_terminator_invariant_helper
-  (buf:Buffer.buffer u32) (p0:u32) (p1:u32{p1 <=^ Buffer.len buf /\ p0 <=^ p1}) (h:mem)
-  = let subseq_size = p1 -^ p0 in
+  (buf:Buffer.buffer uint_32) (p0:uint_32) (p1:uint_32{p1 <= Buffer.len buf /\ p0 <= p1}) (h:mem)
+  = let subseq_size = p1 - p0 in
     let subseq = Buffer.as_seq h (Buffer.gsub buf p0 subseq_size) in
-    forall (i:nat). i < v subseq_size ==> Seq.index subseq i =!= 0ul
+    forall (i:nat). // {:pattern (Seq.index subseq i)} //NS: no pattern here; fixme; this one fails
+      i < v subseq_size ==> Seq.index subseq i =!= 0ul
+//Also tried to write the quantifier in terms of indexing directly on buf, rather than on the subbuf
+//no luck with that either
 
 (* Lifted to hsl_state *)
 [@"opaque_to_smt"]
@@ -82,16 +84,17 @@ unfold private let null_terminator_invariant (st:hsl_state) (h:mem{liveness_and_
     null_terminator_invariant_helper buf p0 p1 h
 
 (*
- * An invariant on the list that all subsequences are 0ul free
+ * An invariant on the list that all subsequences are 0ul free //NS: Can the null_terminator_invariant be phrased as just an instance of this?
  *)
 [@"opaque_to_smt"]
 unfold private let msgs_list_invariant_helper
-  (buf:Buffer.buffer u32) (l:list (u32 * u32)) (p0:u32{p0 <=^ Buffer.len buf}) (h:mem)
-  = forall (i j:u32). List.Tot.mem (i, j) l ==>  //if (i, j) is in the list
-                 (i <^ j /\ j <^ p0 /\  //then both lie before p0
-		  (let subseq_size = j -^ i in
-		   let subseq = Buffer.as_seq h (Buffer.gsub buf i subseq_size) in
-		   forall (k:nat). k < v subseq_size ==> Seq.index subseq k =!= 0ul))  //and no 0ul
+  (buf:Buffer.buffer uint_32) (l:list (uint_32 & uint_32)) (p0:uint_32{p0 <= Buffer.len buf}) (h:mem)
+  = forall ij. //{:pattern (List.Tot.mem ij l)} //NS: fixme; tried this pattern and also separately quantifying i,j; neither worked
+          let i, j = ij in
+          List.Tot.mem ij l ==>  //if (i, j) is in the list
+          (i < j /\
+           j < p0 /\  //then both lie before p0
+           null_terminator_invariant_helper buf i j h)
 
 (* Lifted to hsl_state *)
 [@"opaque_to_smt"]
@@ -123,9 +126,9 @@ let lemma_hsl_invariant_elim (st:hsl_state) (h:mem)
  *)
 let hsl_footprint (st:hsl_state) (h:mem{hsl_invariant st h}) =
   loc_union (loc_union (loc_buffer (Buffer.gsub (hsl_get_buf st) 0ul (sel h (hsl_get_p1 st))))
-		       (loc_mreference (hsl_get_p0 st)))
-	    (loc_union (loc_mreference (hsl_get_p1 st))
-	               (loc_mreference (hsl_get_msgs st)))
+                       (loc_mreference (hsl_get_p0 st)))
+            (loc_union (loc_mreference (hsl_get_p1 st))
+                       (loc_mreference (hsl_get_msgs st)))
 
 (*
  * Framing the HSL invariant across its footprint
@@ -133,22 +136,24 @@ let hsl_footprint (st:hsl_state) (h:mem{hsl_invariant st h}) =
 let lemma_frame_hsl_invariant (st:hsl_state) (l:loc) (h0 h1:mem)
   :Lemma (requires (hsl_invariant st h0                  /\
                     loc_disjoint l (hsl_footprint st h0) /\
-		    Mods.modifies l h0 h1))
-	 (ensures  (hsl_invariant st h1 /\ hsl_footprint st h1 == hsl_footprint st h0))
+                    Mods.modifies l h0 h1))
+         (ensures  (hsl_invariant st h1 /\
+                    hsl_footprint st h1 == hsl_footprint st h0))
   = ()
 
 (*
  * Creating of HSL state
  *)
-let hsl_create (len:u32{len >^ 0ul})
+let hsl_create (len:uint_32{len > 0ul})
   :ST hsl_state (requires (fun h0       -> True))
                 (ensures  (fun h0 st h1 -> Buffer.len (hsl_get_buf st) == len               /\
-		                        hsl_invariant st h1                              /\
-		                        fresh_loc (loc_buffer (hsl_get_buf st)) h0 h1    /\
-					fresh_loc (loc_mreference (hsl_get_p0 st)) h0 h1 /\
-					fresh_loc (loc_mreference (hsl_get_p1 st)) h0 h1 /\
-					fresh_loc (loc_mreference (hsl_get_msgs st)) h0 h1 /\
-		                        Mods.modifies loc_none h0 h1))
+                                        hsl_invariant st h1                              /\
+                                        fresh_loc (loc_buffer (hsl_get_buf st)) h0 h1    /\
+                                        fresh_loc (loc_mreference (hsl_get_p0 st)) h0 h1 /\
+                                        fresh_loc (loc_mreference (hsl_get_p1 st)) h0 h1 /\
+                                        fresh_loc (loc_mreference (hsl_get_msgs st)) h0 h1 /\
+                                        sel h1 (hsl_get_p1 st) == 0ul                    /\
+                                        Mods.modifies loc_none h0 h1))
   = let h0 = ST.get () in
     let buf = Buffer.gcmalloc root 0ul len in
     let h00 = ST.get () in
@@ -165,26 +170,26 @@ let hsl_create (len:u32{len >^ 0ul})
  * Processes the buffer between p1 and p, one at a time
  * Returns new p0, and updated list of indices
  *)
-private let rec aux_process (b:Buffer.buffer u32) (p0 p1 p:u32) (l:list (u32 * u32))
-  :ST (u32 * list (u32 * u32))
+private let rec aux_process (b:Buffer.buffer uint_32) (p0 p1 p:uint_32) (l:list (uint_32 & uint_32))
+  :ST (uint_32 & list (uint_32 & uint_32))
       (requires (fun h0 -> Buffer.live h0 b /\
-                        p <=^ Buffer.len b /\ p1 <=^ p /\ p0 <=^ p1 /\
+                        p <= Buffer.len b /\ p1 <= p /\ p0 <= p1 /\
                         null_terminator_invariant_helper b p0 p1 h0 /\
-			msgs_list_invariant_helper b l p0 h0))
-      (ensures  (fun h0 (r, l) h1 -> Buffer.live h1 b /\ 
-	                          r <=^ p /\
-				  null_terminator_invariant_helper b r p h1 /\
-				  msgs_list_invariant_helper b l r h1 /\
-	                          Mods.modifies loc_none h0 h1))
+                        msgs_list_invariant_helper b l p0 h0))
+      (ensures  (fun h0 (r, l) h1 -> Buffer.live h1 b /\
+                                  r <= p /\
+                                  null_terminator_invariant_helper b r p h1 /\
+                                  msgs_list_invariant_helper b l r h1 /\
+                                  Mods.modifies loc_none h0 h1))
   = if p = p1 then p0, l  //done
     else
       let c = Buffer.index b p1 in
       if c = 0ul then  //found a 0
-        if p0 = p1 then aux_process b (p1 +^ 1ul) (p1 +^ 1ul) p l  //if the subsequence is empty, just go ahead
-        else aux_process b (p1 +^ 1ul) (p1 +^ 1ul) p ((p0, p1)::l)  //else add it to the list
-      else aux_process b p0 (p1 +^ 1ul) p l
+        if p0 = p1 then aux_process b (p1 + 1ul) (p1 + 1ul) p l  //if the subsequence is empty, just go ahead
+        else aux_process b (p1 + 1ul) (p1 + 1ul) p ((p0, p1)::l)  //else add it to the list
+      else aux_process b p0 (p1 + 1ul) p l
 
-#set-options "--z3rlimit 16"
+#reset-options "--max_fuel 0 --max_ifuel 1 --initial_ifuel 1 --z3rlimit 16"
 
 (*
  * Main process function that client (Record) calls once it has appended some data to the input buffer
@@ -192,17 +197,43 @@ private let rec aux_process (b:Buffer.buffer u32) (p0 p1 p:u32) (l:list (u32 * u
  * Also updates the msgs
  * And maintains the invariant
  *)
-let hsl_process (st:hsl_state) (p:u32)
+let hsl_process (st:hsl_state) (p:uint_32)
   :ST unit (requires (fun h0      -> hsl_invariant st h0 /\  //invariant holds
-                                  p <=^ hsl_get_len st /\  //the new index upto which client wrote is in bounds
-				  sel h0 (hsl_get_p1 st) <^ p))  //p1 < p, i.e. some new data is there
+                                  p <= hsl_get_len st /\  //the new index upto which client wrote is in bounds
+                                  sel h0 (hsl_get_p1 st) < p))  //p1 < p, i.e. some new data is there
            (ensures  (fun h0 _ h1 -> hsl_invariant st h1 /\  //invariants holds again
-	                          sel h1 (hsl_get_p1 st) == p /\  //p1 has been updated to p
-	                          Mods.modifies (Mods.loc_union (Mods.loc_mreference (hsl_get_p0 st))
+                                  sel h1 (hsl_get_p1 st) == p /\  //p1 has been updated to p
+                                  Mods.modifies (Mods.loc_union (Mods.loc_mreference (hsl_get_p0 st))
                                                 (Mods.loc_union (Mods.loc_mreference (hsl_get_msgs st))
-				                                (Mods.loc_mreference (hsl_get_p1 st)))) h0 h1))
-  = let len, buf, p0, p1, msgs = hsl_get_len st, hsl_get_buf st, hsl_get_p0 st, hsl_get_p1 st, hsl_get_msgs st in
-    let new_p0, new_msgs = aux_process buf !p0 !p1 p !msgs in
-    p0 := new_p0;
-    p1 := p;
-    msgs := new_msgs
+                                                                (Mods.loc_mreference (hsl_get_p1 st)))) h0 h1))
+  = let new_p0, new_msgs = aux_process st.buf !st.p0 !st.p1 p !st.msgs in
+    st.p0 := new_p0;
+    st.p1 := p;
+    st.msgs := new_msgs
+
+#set-options "--z3rlimit_factor 2"
+let top_level () : St unit =
+  let st = hsl_create 128ul in
+  let buf = hsl_get_buf st in
+  let rec aux (i:uint_32)
+    : ST unit
+      (requires (fun h ->
+        let p1 = sel h (hsl_get_p1 st) in
+        hsl_get_len st == 128ul /\         //not sure why I need this as a precondition
+        hsl_invariant st h /\
+        p1 <= i /\
+        i <= hsl_get_len st /\
+        (p1 <> i ==> null_terminator_invariant_helper buf (p1 + 1ul) i h)))
+      (ensures fun h0 _ h1 ->
+        hsl_invariant st h1
+      )
+    = let p1 = !st.p1 in
+      if i = hsl_get_len st then ()
+      else if i = 2ul * p1
+      then (buf.(i) <- 0ul;
+            hsl_process st (i + 1ul);
+            aux (i + 1ul))
+      else (buf.(i) <- 1ul;
+            aux (i + 1ul))
+  in
+  aux 0ul
